CoqOfRust/revm/revm_interpreter/links/interpreter.v
@@ -4,7 +4,11 @@ Require Import revm.links.dependencies.
 Require Import revm_interpreter.interpreter.links.shared_memory.
 Require Import revm_interpreter.interpreter.links.stack.
 Require Import revm_interpreter.links.gas.
+Require Import revm_interpreter.links.interpreter_action.
 Require Import revm_interpreter.links.interpreter_types.
+Require Import revm_interpreter.interpreter.
+
+Import Run.
 
 (*
 pub struct Interpreter<WIRE: InterpreterTypes> {
@@ -235,3 +239,79 @@ Module Interpreter.
   Proof. now constructor. Qed.
   Smpl Add apply get_extend_is_valid : run_sub_pointer.
 End Interpreter.
+
+(* impl<IW: InterpreterTypes> Interpreter<IW> { *)
+Module Impl_Interpreter.
+  Definition Self
+    (IW : Set) `{Link IW}
+    {IW_types : InterpreterTypes.Types.t} `{InterpreterTypes.Types.AreLinks IW_types}
+    (run_InterpreterTypes_for_IW : InterpreterTypes.Run IW IW_types) :
+    Set :=
+    Interpreter.t IW IW_types.
+
+  (*
+  pub fn run<FN, H: Host>(
+      &mut self,
+      instruction_table: &[FN; 256],
+      host: &mut H,
+  ) -> InterpreterAction
+  where
+      FN: CustomInstruction<Wire = IW, Host = H>,
+  *)
+  Definition run_run
+      (IW : Set) `{Link IW}
+      {IW_types : InterpreterTypes.Types.t} `{InterpreterTypes.Types.AreLinks IW_types}
+      (run_InterpreterTypes_for_IW : InterpreterTypes.Run IW IW_types)
+      (FN : Set) `{Link FN}
+      (H_ : Set) `{Link H_}
+      (self : Ref.t Pointer.Kind.MutRef (Self IW run_InterpreterTypes_for_IW))
+      (instruction_table : Ref.t Pointer.Kind.Ref (array.t FN {| Integer.value := 256 |}))
+      (host : Ref.t Pointer.Kind.MutRef H_) :
+    {{
+      interpreter.Impl_revm_interpreter_interpreter_Interpreter_IW.run
+        (Φ IW)
+        []
+        [ Φ FN; Φ H_ ]
+        [ φ self; φ instruction_table; φ host ] 🔽
+      InterpreterAction.t
+    }}.
+  Proof.
+    run_symbolic.
+    eapply Run.Rewrite. {
+      erewrite IsTraitAssociatedType_eq by apply run_InterpreterTypes_for_IW.
+      reflexivity.
+    }
+    run_symbolic_let. {
+      destruct run_InterpreterTypes_for_IW.
+      destruct run_LoopControl_for_Control.
+      destruct set_next_action as [set_next_action [H_set_next_action run_set_next_action]].
+      run_symbolic.
+    }
+    intros [|[]]; run_symbolic.
+    run_symbolic_let. {
+      admit.
+    }
+    intros [|[]]; run_symbolic.
+    run_symbolic_let. {
+      destruct run_InterpreterTypes_for_IW.
+      destruct run_LoopControl_for_Control.
+      destruct take_next_action as [take_next_action [H_take_next_action run_take_next_action]].
+      run_symbolic.
+    }
+    intros [|[]]; run_symbolic.
+    run_symbolic_let. {
+      run_symbolic.
+      run_symbolic_closure. {
+        apply Impl_InterpreterAction.run_is_some.
+      }
+      intros []; run_symbolic.
+      run_symbolic_are_equal_bool; run_symbolic.
+    }
+    intros [|[]]; run_symbolic.
+    destruct run_InterpreterTypes_for_IW.
+    destruct run_LoopControl_for_Control.
+    destruct instruction_result as [instruction_result [H_instruction_result run_instruction_result]].
+    run_symbolic.
+    admit.
+  Admitted.
+End Impl_Interpreter.
